# Cubic Spline

We consider here a cubic spline passing through the points ``(x_i,y_i)`` with ``a=x_1<\ldots<x_n=b``, that is, a class function ``{\mathcal C}^2`` on ``[a, b]`` and each restriction at the interval ``[x_{i-1},x_i]``, ``1\leq i\leq n``, is a polynomial of degree less than 3. We will note ``S`` such a spline. His equation is given by

```math
    S_i(x) =  Ay_i + By_{i+1} + Cy''_i+ D y''_{i+1}, \qquad x_{i}\leq x\leq x_{i+1},
```

where

```math
    A = \frac{x_{i+1}-x}{x_{i+1} - x_i} \qquad \text{et} \qquad B = \frac{x-x_i}{x_{i+1} - x_i},
```

```math
    C = \frac{1}{6}\left(A^3-A\right)\left(x_{i+1}-x_i\right)^2 \qquad \text{et} \qquad D = \frac{1}{6}\left(B^3-B\right)\left(x_{i+1}-x_i\right)^2.
```

If we derive this equation twice with respect to :math:`x`, we get

```math
    \frac{d^2S(x)}{d x} = Ay''_i + By''_{i+1}.
```

Since ``A = 1`` in ``x_i`` and ``A = 0`` in ``x_ {i + 1}`` and conversely for ``B``, we can see that the second derivative is continuous at the interface of the two intervals ``[x_{i-1}, x_{i}]`` and ``[x_{i}, x_{i + 1}]``.

It remains to determine the expression of ``y''_i``. To do this, we will calculate the first derivative and impose that it is continuous at the interface of two intervals. The first derivative is given by

```math
    \frac{dy}{dx}=\frac{y_{i+1}-y_{i}}{x_{i+1}-x_{i}}-\frac{3A^2-1}{6}(x_{i+1}-x_{i})y''_i+\frac{3B^2-1}{6}(x_{i+1}-x_{i})y''_{i+1}.
```

We therefore want the value of the first derivative in ``x = x_i`` over the interval ``[x_{i-1}, x_{i}]`` to be equal to the value of the first derivative in ``x = x_i`` over the interval ``[x_{i}, x_{i + 1}]``; which gives us for ``i = 2, \dots, n-1``

```math
    a_iy''_{i-1}+b_iy''_i+c_iy''_{i+1}=d_i,
```

with

```math
    \begin{array}{l}
    a_i = \frac{x_i-x_{i-1}}{x_{i+1}-x_{i-1}}\\
    b_i = 2\\
    c_i = \frac{x_{i+1}-x_{i}}{x_{i+1}-x_{i-1}}\\
    d_i = \frac{6}{x_{i+1}-x_{i-1}}\left(\frac{y_{i+1}-y_{i}}{x_{i+1}-x_{i}}-\frac{y_{i}-y_{i-1}}{x_{i}-x_{i-1}}\right).
    \end{array}
```

So we have ``n-2`` linear equations to calculate the ``n`` unknowns ``y''_i`` for ``i = 1, \dots, n``. So we have to make a choice for the first and last values and we will take them equal to zero. We can recognize the resolution of a system with a tridiagonal matrix. It is then easy to solve it by using the algorithm of Thomas which one recalls the principle

```math
    c'_i=\left\{
    \begin{array}{lr}
    \frac{ci}{b_i}&i=1\\
    \frac{c_i}{b_i-a_ic'_{i-1}}&i=2,\dots,n.
    \end{array}
    \right.
```

```math
    d'_i=\left\{
    \begin{array}{lr}
    \frac{di}{b_i}&i=1\\
    \frac{d_i-a_id'_{i-1}}{b_i-a_ic'_{i-1}}&i=2,\dots,n.
    \end{array}
    \right.
```

The solution is then obtained by the formula

```math
    \begin{array}{l}
    y''_n = d'_n \\
    y''_i = d'_i-c'_iy''_{i+1} \qquad \text{for} \qquad i=n-1,\dots,1.
    \end{array}
```
